\documentclass[a4paper,11pt]{article}
\usepackage{psfrag}
\usepackage[english,greek]{babel}
\usepackage[iso-8859-7]{inputenc}
\usepackage{amssymb}
\usepackage{amsmath}
\usepackage[T1]{fontenc}
\usepackage{txfontsb}
\usepackage[lite]{mtpro2}
\usepackage[left=2.00cm, right=2.00cm, top=3.00cm, bottom=3.00cm]{geometry}
\usepackage{tikz}
\usepackage{tkz-euclide,tkz-fct}
\usepackage{wrapfig}
\usetkzobj{all}
\usepackage{calc}
\usepackage[framemethod=TikZ]{mdframed}

\usepackage{titletoc}
\usepackage[explicit]{titlesec}
\usepackage{graphicx}
\usepackage{multicol}
\usepackage{multirow}
\usepackage{enumitem}
\usepackage{tabularx}
\usepackage[decimalsymbol=comma]{siunitx}
\usetikzlibrary{backgrounds}
\usepackage{sectsty}
\sectionfont{\centering}

\begin{document}
\section*{\textcolor{black}{{\LARGE ΕΞΙΣΩΣΕΙΣ}}}
\begin{center}
{\normalsize  \bf\today}\mbox{}\\
\vspace{5mm}
\textcolor{black}{\textbf{{\large ΚΛΑΣΜΑΤΙΚΕΣ ΕΞΙΣΩΣΕΙΣ}}}
\end{center}
\paragraph{\textcolor{black}{{\large ΑΣΚΗΣΕΙΣ}}}\mbox{}\\
\begin{enumerate}[label=\bf\textcolor{black}{{\large \arabic*.}},
itemsep=5mm]
\item Να λυθούν οι παρακάτω εξισώσεις.
\begin{multicols}{3}
\begin{enumerate}[label=\roman*.]
\item $ \dfrac{4}{x-1}=\dfrac{2}{x} $
\item $ \dfrac{5}{2x+3}=\dfrac{4}{x-3} $
\item $ \dfrac{2}{4x+3}=\dfrac{3}{x-3} $
\item $ \dfrac{x}{3-x}=\dfrac{4}{x} $
\item $ \dfrac{x+2}{3x-1}=\dfrac{x-2}{2x+1} $
\item $ \dfrac{3x}{x-2}=\dfrac{x-2}{3x} $
\end{enumerate}
\end{multicols}
\item Να λυθούν οι παρακάτω εξισώσεις.
\begin{multicols}{3}
\begin{enumerate}[label=\roman*.]
\item $ \dfrac{x}{x-1}+\dfrac{x-2}{x}=2 $
\item $ \dfrac{x}{x+1}+\dfrac{2}{x-1}=1 $
\item $ \dfrac{x+1}{x}+\dfrac{4}{x-3}=\dfrac{1}{x} $
\item $ \dfrac{2}{x-2}=\dfrac{1}{x}-\dfrac{3}{x^2} $
\item $ \dfrac{3}{x-1}=\dfrac{x}{(x-1)^2}-1 $
\item $ \dfrac{3}{x-4}-\dfrac{x}{x+4}=-1 $
\end{enumerate}
\end{multicols}
\item Να λυθούν οι παρακάτω εξισώσεις.
\begin{multicols}{2}
\begin{enumerate}[label=\roman*.]
\item $ \dfrac{1}{x-2}-\dfrac{x}{x+2}=\dfrac{2 x}{x^2-4} $
\item $ \dfrac{x-2}{x^2-1}-\dfrac{x}{x-1}=\dfrac{2}{x+1} $
\item $ \dfrac{x}{4x^2-9}-\dfrac{1-3x}{2x-3}=\dfrac{1}{2x+3} $
\item $ \dfrac{x-5}{x^2-25}=\dfrac{4}{x-5}-\dfrac{1}{x+5} $
\item $ \dfrac{3}{x-3}=\dfrac{4}{x^2-9}-1 $
\item $ \dfrac{2 x}{x-4}-\dfrac{3-x}{x^2-16}=\dfrac{1-x}{x+4} $
\end{enumerate}
\end{multicols}
\item Να λυθούν οι παρακάτω εξισώσεις.
\begin{multicols}{2}
\begin{enumerate}[label=\roman*.]
\item $ \dfrac{2}{x-2}-\dfrac{x}{x^2-2 x}=\dfrac{3}{x} $
\item $ \dfrac{1-x}{x}+\dfrac{1}{x-3}=\dfrac{3}{x^2-3 x} $
\item $ \dfrac{x-1}{x+4}+\dfrac{2-x}{x}=\dfrac{1-x}{x^2+4 x}+1 $
\item $  $
\end{enumerate}
\end{multicols}
\end{enumerate}
\end{document}