%# File Id : Ana-DiafL-ParSyn-PrPrf5-1
%@ FilesDB Id : G_Epal
Θεωρούμε τη συνάρτηση $ F(x)=f(x)+g(x) $ με $ x\in A $. Έχουμε ότι
\[ F(x+h)-F(x)=f(x+h)+g(x+h)-(f(x)+g(x))=f(x+h)-f(x)+g(x+h)-g(x) \]
Για κάθε $ h\neq 0 $ ισχύει
\[ \frac{F(x+h)-F(x)}{h}=\frac{f(x+h)-f(x)+g(x+h)-g(x)}{h}=\frac{f(x+h)-f(x)}{h}+\frac{g(x+h)-g(x)}{h} \]
άρα
\[ \lim_{h\to 0}\frac{F(x+h)-F(x)}{h}=\lim_{h\to 0}\frac{f(x+h)-f(x)}{h}+\lim_{h\to 0}\frac{g(x+h)-g(x)}{h}=f'(x)+g'(x) \]
Οπότε $ (f(x)+g(x))'=f'(x)+g'(x) $ για κάθε $ x\in A $.
%# End of file Ana-DiafL-ParSyn-PrPrf5-1