%# Database File : DTX-Geometria-KwnT-ExisKyklou-ExKyklou-SolSE4-1
%@ Database source: Mathematics
\begin{alist}
\item Με κέντρο $ K(2,-3) $ και ακτίνα $ \rho=4 $ ο κύκλος έχει εξίσωση
\[ (x-x_K)^2+(y-y_K)^2=\rho^2\Rightarrow (x-2)^2+(y-(-3))^2=4^2\Rightarrow (x-2)^2+(y+3)^2=16 \]
\item $ (x-x_K)^2+(y-y_K)^2=\rho^2\Rightarrow (x-(-4))^2+(y-5)^2=3^2\Rightarrow (x+4)^2+(y-5)^2=9 $
\item $ (x-x_K)^2+(y-y_K)^2=\rho^2\Rightarrow (x-1)^2+(y-1)^2=\sqrt{5}^2\Rightarrow (x-1)^2+(y-1)^2=5 $
\item $ (x-x_K)^2+(y-y_K)^2=\rho^2\Rightarrow (x-0)^2+(y-(-2))^2=\left(\frac{1}{2}\right)^2\Rightarrow x^2+(y+2)^2=\frac{1}{4} $
\item $ (x-x_K)^2+(y-y_K)^2=\rho^2\Rightarrow (x-7)^2+(y-0)^2=\left(\frac{\sqrt{3}}{3}\right)^2\Rightarrow (x-7)^2+y^2=\frac{1}{3} $
\item $ (x-x_K)^2+(y-y_K)^2=\rho^2\Rightarrow \left(x-\frac{3}{2}\right)^2+\left(y-\frac{1}{2}\right)^2=1^2\Rightarrow \left(x-\frac{3}{2}\right)^2+\left(y-\frac{1}{2}\right)^2=1 $
\end{alist}
%# End of file DTX-Geometria-KwnT-ExisKyklou-ExKyklou-SolSE4-1